worked on proof of lemma 18

HML_Attack_Formulas.thy
@@ -11,6 +11,42 @@ for
   \<tau> :: \<open>'a\<close>
 begin
 
+fun is_dist ::  \<open>('a,'s) HML_formula \<Rightarrow> 's \<Rightarrow> 's \<Rightarrow> bool\<close>
+  where
+   \<open>is_dist \<phi> p q = (p \<Turnstile> \<phi> \<and> \<not> q \<Turnstile> \<phi>)\<close>
+
+fun is_dist_set ::  \<open>('a,'s) HML_formula \<Rightarrow> 's \<Rightarrow> 's set \<Rightarrow> bool\<close>
+  where
+   \<open>is_dist_set \<phi> p Q = (p \<Turnstile> \<phi> \<and> (\<forall>q. q \<in> Q \<longrightarrow> \<not> q \<Turnstile> \<phi>))\<close>
+
+
+lemma all_states_sat_empty_conjunction:
+  shows \<open>\<forall>q. q \<Turnstile> (HML_weaknor {} (\<lambda>i. HML_true))\<close>
+proof - 
+  have \<open>\<forall>q F. q \<Turnstile> (HML_conj {} (\<lambda>f. HML_neg (F f)))\<close> by auto
+  thus ?thesis                     
+    by (metis HML_formula.distinct(9, 11)
+        HML_formula.inject(3) HML_weaknor_def satisfies.elims(3) step_tau_refl tau_def)
+qed
+
+lemma tau_a_obs_implies_delay_step: 
+  assumes \<open>p  \<Turnstile> \<langle>\<tau>\<rangle>\<langle>a\<rangle>\<phi>\<close>
+  shows \<open>\<exists>p'. p =\<rhd>a p' \<and> p' \<Turnstile> \<phi>\<close>
+proof - 
+  obtain p'' where \<open>p \<Rightarrow>^\<tau> p'' \<and> p'' \<Turnstile> \<langle>a\<rangle>\<phi>\<close> using assms by auto
+  thus ?thesis using satisfies.simps(4) steps_concat tau_tau by blast
+qed
+
+lemma delay_step_implies_tau_a_obs: 
+  assumes 
+    \<open>p =\<rhd>a p'\<close>
+    \<open>p' \<Turnstile> \<phi>\<close>
+  shows \<open>p  \<Turnstile> \<langle>\<tau>\<rangle>\<langle>a\<rangle>\<phi>\<close>
+proof - 
+  obtain p'' where \<open>p \<Rightarrow>^\<tau> p''\<close> and \<open>p'' \<Rightarrow>^a p'\<close> using assms steps.refl tau_tau by blast
+  thus ?thesis by (metis assms(1,2) lts_tau.satisfies.simps(4) lts_tau.tau_tau)
+qed
+
 function wr ::  \<open>('s, 'a) c_set_game_node \<Rightarrow> bool\<close> 
   where 
     \<open>wr (DefenderSwapNode p Q) = (if Q = {} then True
@@ -22,65 +58,119 @@ function wr ::  \<open>('s, 'a) c_set_game_node \<Rightarrow> bool\<close>
        apply simp+
   done
 
-
-fun is_dist ::  \<open>('a,'s) HML_formula \<Rightarrow> 's \<Rightarrow> 's \<Rightarrow> bool\<close>
-  where
-   \<open>is_dist \<phi> p q = (p \<Turnstile> \<phi> \<and> \<not> q \<Turnstile> \<phi>)\<close>
-
-
-lemma all_states_sat_empty_conjunction:
-  shows \<open>\<forall>q. q \<Turnstile> (HML_weaknor {} (\<lambda>i. HML_true))\<close>
-proof - 
-  have \<open>\<forall>q F. q \<Turnstile> (HML_conj {} (\<lambda>f. HML_neg (F f)))\<close> by auto
-  thus ?thesis
-    by (metis HML_formula.distinct(9, 11)
-        HML_formula.inject(3) HML_weaknor_def satisfies.elims(3) step_tau_refl tau_def)
-qed
-
-lemma tau_a_obs_implies_delay_step: 
-  assumes \<open>p  \<Turnstile> \<langle>\<tau>\<rangle>\<langle>a\<rangle>\<phi>\<close>
-  shows \<open>\<exists>p'. p =\<rhd>a p' \<and> p' \<Turnstile> \<phi>\<close>
-proof - 
-  obtain p'' where \<open>p \<Rightarrow>^\<tau> p'' \<and> p'' \<Turnstile> \<langle>a\<rangle>\<phi>\<close>
-    using assms 
-    by auto
-  thus ?thesis
-    using satisfies.simps(4) steps_concat tau_tau by blast
-qed
-
-
-lemma dist_formula_implies_wr_inclusion: 
-  assumes \<open>\<phi> \<in> HML_weak_formulas\<close>
-  shows \<open>\<forall>q. q \<in> Q \<and> (is_dist \<phi> p q) \<Longrightarrow> wr (AttackerNode p Q)\<close>
-proof (induct arbitrary: p Q rule: HML_weak_formulas.induct[OF assms])
-  case Base: 1
-  have \<open>\<forall>q. q \<Turnstile> (HML_weaknor {} (\<lambda>i. HML_true))\<close>
-    by (simp add: all_states_sat_empty_conjunction)
-  then show ?case
-    using Base is_dist.elims(2) by blast
-next
-  case Obs: (2 \<phi> a)
-  thus ?case 
-    by (meson is_dist.elims(2))
-next
-  case Conj: (3 I F)
-  then show ?case by auto
-qed
-
 fun atk_strat :: \<open>('s, 'a) c_set_game_node list \<Rightarrow> ('s, 'a) c_set_game_node\<close>
   where 
 \<open>atk_strat ((AttackerNode p Q)#play) = 
 (SOME g'. c_set_game_moves (AttackerNode p Q) g' \<and> wr g')\<close>
 | \<open>atk_strat _ = undefined\<close>
 
-
-
+(*
 lemma attacker_wins_in_winning_region: 
   assumes \<open>wr (AttackerNode p Q)\<close>
   shows \<open>player1_winning_strategy atk_strat (AttackerNode p Q)\<close>
   (*unfolding player1_winning_strategy_def*)
 proof -
+  obtain g where \<open>c_set_game_moves (AttackerNode p Q) g \<and> wr g\<close> using assms sledgehammer
   show ?thesis sorry
 qed
+*)
+thm HML_weak_formulas.induct
+
+
+lemma tau_obs_implies_delay: 
+  assumes 
+    \<open>q \<Rightarrow>^\<tau> q'\<close> 
+    \<open>q' \<longmapsto>a q''\<close>
+  shows \<open>q =\<rhd>a q''\<close>
+proof -
+  have \<open>q  \<longmapsto>* tau q' \<and> q'  \<longmapsto>a q''\<close> using assms by auto
+  then show ?thesis
+    using steps.step by blast
+qed
+
+lemma Atk_node_wins_if_Q_is_empty: 
+  assumes \<open>Q = {}\<close>
+  shows \<open>wr (AttackerNode p Q)\<close>
+proof - 
+  have \<open>c_set_game_moves (AttackerNode p Q) (DefenderSwapNode p Q)\<close> 
+    by (simp add: steps.refl)
+  have \<open>wr (DefenderSwapNode p Q)\<close> using assms sorry
+  thus ?thesis sorry
+qed
+
+
+lemma Atk_node_wins_in_2_moves: 
+  assumes 
+        \<open>wr (AttackerNode p' (dsuccs a Q))\<close>
+        \<open>p =\<rhd>a p'\<close>
+  shows \<open>wr (AttackerNode p Q)\<close>
+proof - 
+  oops
+
+
+lemma dist_formula_implies_wr_inclusion: 
+  assumes 
+    \<open>\<phi> \<in> HML_weak_formulas\<close>
+    \<open>is_dist_set \<phi> p Q\<close>
+  shows \<open>wr (AttackerNode p Q)\<close>
+  (*shows \<open>\<forall>q. q \<in> Q \<and> (is_dist \<phi> p q) \<longrightarrow> wr (AttackerNode p Q)\<close>*)
+proof(cases \<open>Q = {}\<close>)
+  case True
+  then show ?thesis using Atk_node_wins_if_Q_is_empty by auto
+next
+  case False
+  then show ?thesis using assms
+  proof (induct arbitrary: p Q rule: HML_weak_formulas.induct[OF assms(1)])
+    case Base: 1
+    have \<open>\<forall>q. q \<Turnstile> (HML_weaknor {} (\<lambda>i. HML_true))\<close>
+      by (simp add: all_states_sat_empty_conjunction)
+    hence \<open>False\<close> 
+      using Base.prems(1, 3) by simp
+    then show ?case by auto
+  next
+    case Obs: (2 \<phi> a)
+    then obtain p' where p'_def: \<open>p =\<rhd>a p' \<and> p' \<Turnstile> \<phi> \<close> 
+      using tau_a_obs_implies_delay_step[of p a \<phi>] by auto
+    have \<open>\<forall>q. q \<in> Q \<longrightarrow> \<not> q \<Turnstile> \<langle>\<tau>\<rangle>\<langle>a\<rangle>\<phi>\<close> using Obs by auto
+    hence \<open>\<forall>q. q \<in> Q \<longrightarrow> (\<forall>q'.  \<not>q  =\<rhd>a  q' \<or> \<not>q' \<Turnstile> \<phi>)\<close>
+      using delay_step_implies_tau_a_obs by blast
+    hence \<open>\<forall>q'. q' \<in> dsuccs a Q \<longrightarrow> \<not> q' \<Turnstile> \<phi>\<close> 
+      unfolding dsuccs_def by blast
+    hence phi_distinguishing: \<open>is_dist_set \<phi> p' (dsuccs a Q)\<close> 
+      using p'_def by simp
+(*
+    hence \<open>wr (AttackerNode p' (dsuccs a Q))\<close>*)
+    thus ?case
+    proof (cases \<open>dsuccs a Q = {}\<close>)
+      case dsuccs_empty: True
+      then show ?thesis
+      proof (cases \<open>tau a\<close>)
+        case True
+        hence \<open>{q1. \<exists>q\<in> Q. q \<longmapsto>* tau q1} = {}\<close> using dsuccs_def dsuccs_empty by auto
+        hence \<open>Q = {}\<close> using steps.refl by blast
+        then show ?thesis using Atk_node_wins_if_Q_is_empty by auto
+      next
+        case False
+        hence AtkToSim: \<open>c_set_game_moves (AttackerNode p Q) (DefenderSimNode a p' Q)\<close>
+          using p'_def by simp
+        have SimToAtk: \<open>\<forall>g. c_set_game_moves 
+(DefenderSimNode a p' Q) g \<longrightarrow> (g = AttackerNode p' (dsuccs a Q))\<close>
+          by (metis c_set_game.move_DefSim_to_AtkNode)
+        hence \<open>wr (AttackerNode p' (dsuccs a Q))\<close> 
+          using Atk_node_wins_if_Q_is_empty dsuccs_empty by auto
+        hence \<open>wr (DefenderSimNode a p' Q)\<close>  using SimToAtk sorry
+        thus \<open>wr (AttackerNode p Q)\<close>  using AtkToSim sorry
+      qed
+    next
+      case dsuccs_nonempty: False
+      hence \<open>wr (AttackerNode p' (dsuccs a Q))\<close> using Obs.hyps phi_distinguishing by auto
+      thus ?thesis sorry
+    qed
+  next
+    case Conj: (3 I F)
+    then show ?case sorry
+  qed
+qed
+
 end
 end
